\documentclass{article}
\usepackage{amsthm}
\usepackage{amsmath}
\usepackage{amssymb}
\newtheorem{lemma}{Lemma}
\begin{document}
	\title{A proof of Minkowski’s inequality}
	\maketitle
\begin{flushleft}
	Suppose that $n \in\mathbb{N}$, and let $a_{k}, b_{k} \in\mathbb{R}, 1\leq k\leq n$. If $1<p<\infty$ and $\frac{1}{p}+\frac{1}{q}=1$ then\[\left[\sum_{k=1}^{n} \left|a_{k}+b_{k}\right|^{p}\right]^{\frac{1}{p}}\leq \left[\sum_{k=1}^{n} \left|a_{k}\right|^{p}\right]^{\frac{1}{p}}+\left[\sum_{k=1}^{n} \left|b_{k}\right|^{p}\right]^{\frac{1}{p}}\]
\end{flushleft}
\begin{proof}
	~\\
	\linespread{1.5}
	We first show the $H\ddot{o}lder’s\ inequality$ under assumption.
	\[\sum_{k=1}^{n}\left|a_{k}b_{k}\right| \leq \left[\sum_{k=1}^{n} \left|a_{k}\right|^{p}\right]^{\frac{1}{p}}\left[\sum_{k=1}^{n} \left|b_{k}\right|^{p}\right]^{\frac{1}{p}}\]
	\begin{lemma}
		If $A,B>0$ and $t<1$, then $A^{t}B^{1-t}\leq tA+(1-t)B$
		\begin{proof}
			~\\
			Define $f(A)=tA+(1-t)B-A^{t}B^{1-t}$\\
			let $\frac{\partial}{\partial A}f=t-tA^{t-1}B^{1-t}=0$\\
			Notice $\frac{\partial ^{2}}{\partial A^{2}}f=-t(t-1)A^{t-2}B^{1-t}>0$\\
			Thus $f$ has a minimum at $A=B$
		\end{proof}
	\end{lemma}
	Thus\\
	\begin{align*}
		\frac{\sum_{k=1}^{n}\left|a_{k}b_{k}\right|}{\left[\sum_{k=1}^{n} \left|a_{k}\right|^{p}\right]^{\frac{1}{p}}\left[\sum_{k=1}^{n} \left|b_{k}\right|^{p}\right]^{\frac{1}{p}}} 
		    &= \sum_{k=1}^{n} \frac{(\left|a_{k}\right|^{p})^{\frac{1}{p}}}{\left[\sum_{k=1}^{n} \left|a_{k}\right|^{p}\right]^{\frac{1}{p}}}\frac{(\left|b_{k}\right|^{q})^{\frac{1}{q}}}{\left[\sum_{k=1}^{n} \left|b_{k}\right|^{q}\right]^{\frac{1}{q}}}\\
			&\leq  \sum_{k=1}^{n} \frac{(\left|a_{k}\right|^{p})}{p\left[\sum_{k=1}^{n} \left|a_{k}\right|^{p}\right]}+\frac{(\left|b_{k}\right|^{q})}{q\left[\sum_{k=1}^{n} \left|b_{k}\right|^{q}\right]} \\
		    &=\frac{1}{p}+\frac{1}{q}=1
	\end{align*}
	We now prove Minkowski’s inequality.\\
	By triangle inequality,
	\begin{align*}
		\sum_{k=1}^{n}\left|a_{k}+b_{k}\right|^{p} &\leq \sum_{k=1}^{n}\left|a\right|\left|a_{k}+b_{k}\right|^{p-1}+\sum_{k=1}^{n}\left|b\right|\left|a_{k}+b_{k}\right|^{p-1} \\
		&\leq \left[\sum_{k=1}^{n}\left|a_{k}\right|^{p} \right]^{\frac{1}{p}}\left[\sum_{k=1}^{n}\left|a_{k}+b_{k}\right|^{q(p-1)} \right]^{\frac{1}{q}} + \left[\sum_{k=1}^{n}\left|b_{k}\right|^{p} \right]^{\frac{1}{p}}\left[\sum_{k=1}^{n}\left|a_{k}+b_{k}\right|^{q(p-1)} \right]^{\frac{1}{q}}\\
		&= (\left[\sum_{k=1}^{n}\left|a_{k}\right|^{p} \right]^{\frac{1}{p}}+\left[\sum_{k=1}^{n}\left|b_{k}\right|^{p} \right]^{\frac{1}{p}})\left[\sum_{k=1}^{n}\left|a_{k}+b_{k}\right|^{q(p-1)} \right]^{\frac{1}{q}}\ (*)	
	\end{align*} 
	Note that $\frac{1}{p}+\frac{1}{q}=1 \Rightarrow pq=p+q$\\
	Then
	\begin{align*}
		(*)=(\left[\sum_{k=1}^{n}\left|a_{k}\right|^{p} \right]^{\frac{1}{p}}+\left[\sum_{k=1}^{n}\left|b_{k}\right|^{p} \right]^{\frac{1}{p}})\left[\sum_{k=1}^{n}\left|a_{k}+b_{k}\right|^{p} \right]^{\frac{1}{q}}
	\end{align*}
	That's to say, 
	\begin{align*}
		\sum_{k=1}^{n}\left|a_{k}+b_{k}\right|^{p} \leq (\left[\sum_{k=1}^{n}\left|a_{k}\right|^{p} \right]^{\frac{1}{p}}+\left[\sum_{k=1}^{n}\left|b_{k}\right|^{p} \right]^{\frac{1}{p}})\left[\sum_{k=1}^{n}\left|a_{k}+b_{k}\right|^{p} \right]^{\frac{1}{q}}
	\end{align*}
	Thus, 
	\begin{align*}
		\left[\sum_{k=1}^{n} \left|a_{k}+b_{k}\right|^{p}\right]^{\frac{1}{p}}\leq \left[\sum_{k=1}^{n} \left|a_{k}\right|^{p}\right]^{\frac{1}{p}}+\left[\sum_{k=1}^{n} \left|b_{k}\right|^{p}\right]^{\frac{1}{p}}
	\end{align*}
\end{proof}
\end{document}